src/study/Nemonuri.Study.CSharpSyntaxRewriter2.Modifier2/Nemonuri.StratifiedNodes.Forall.Aggregating.fst
@@ -1,0 +1,28 @@
+module Nemonuri.StratifiedNodes.Forall.Aggregating
+
+module L = FStar.List.Tot
+module N = Nemonuri.StratifiedNodes.Nodes
+module T = Nemonuri.StratifiedNodes.Children.Types
+module C = Nemonuri.StratifiedNodes.Children
+module Common = Nemonuri.StratifiedNodes.Common
+
+//--- members ---
+
+let for_all_aggregator
+  : (Common.aggregator bool) =
+  fun v1 v2 -> (v1 && v2)
+
+let for_all_continue_predicate (t:eqtype)
+  : (C.continue_predicate t bool) 
+  =
+  fun n v -> v
+
+//---|
+
+//--- propositions ---
+
+//---|
+
+//--- proof ---
+
+//---|
